thys/Jinja/JVM/JVMDefensive.thy
@@ -1,5 +1,5 @@
 (*  Title:      HOL/MicroJava/JVM/JVMDefensive.thy
-    ID:         $Id: JVMDefensive.thy,v 1.3 2007-02-07 17:19:08 stefanberghofer Exp $
+    ID:         $Id: JVMDefensive.thy,v 1.4 2007-07-11 10:17:12 stefanberghofer Exp $
     Author:     Gerwin Klein
     Copyright   GPL
 *)
@@ -133,12 +133,14 @@ constdefs
   "exec_d P \<sigma> \<equiv> if check P \<sigma> then Normal (exec (P, \<sigma>)) else TypeError"
 
 
-inductive2
-  "exec_1_d" :: "jvm_prog \<Rightarrow> jvm_state type_error \<Rightarrow> jvm_state type_error \<Rightarrow> bool" 
+inductive_set
+  exec_1_d :: "jvm_prog \<Rightarrow> (jvm_state type_error \<times> jvm_state type_error) set" 
+  and exec_1_d' :: "jvm_prog \<Rightarrow> jvm_state type_error \<Rightarrow> jvm_state type_error \<Rightarrow> bool" 
                    ("_ \<turnstile> _ -jvmd\<rightarrow>\<^isub>1 _" [61,61,61]60)
   for P :: jvm_prog
 where
-  exec_1_d_ErrorI: "exec_d P \<sigma> = TypeError \<Longrightarrow> P \<turnstile> Normal \<sigma> -jvmd\<rightarrow>\<^isub>1 TypeError"
+  "P \<turnstile> \<sigma> -jvmd\<rightarrow>\<^isub>1 \<sigma>' \<equiv> (\<sigma>,\<sigma>') \<in> exec_1_d P"
+| exec_1_d_ErrorI: "exec_d P \<sigma> = TypeError \<Longrightarrow> P \<turnstile> Normal \<sigma> -jvmd\<rightarrow>\<^isub>1 TypeError"
 | exec_1_d_NormalI: "exec_d P \<sigma> = Normal (Some \<sigma>') \<Longrightarrow> P \<turnstile> Normal \<sigma> -jvmd\<rightarrow>\<^isub>1 Normal \<sigma>'"
 
 -- "reflexive transitive closure:"
@@ -149,11 +151,11 @@ syntax (xsymbols)
   "exec_all_d" :: "jvm_prog \<Rightarrow> jvm_state type_error \<Rightarrow> jvm_state type_error \<Rightarrow> bool" 
                    ("_ \<turnstile> _ -jvmd\<rightarrow> _" [61,61,61]60)  
 defs
-  exec_all_d_def1: "P \<turnstile> \<sigma> -jvmd\<rightarrow> \<sigma>' \<equiv> (exec_1_d P)\<^sup>*\<^sup>* \<sigma> \<sigma>'"
+  exec_all_d_def1: "P \<turnstile> \<sigma> -jvmd\<rightarrow> \<sigma>' \<equiv> (\<sigma>,\<sigma>') \<in> (exec_1_d P)\<^sup>*"
 
 lemma exec_1_d_def:
-  "exec_1_d P s t = ((\<exists>\<sigma>. s = Normal \<sigma> \<and> t = TypeError \<and> exec_d P \<sigma> = TypeError) \<or>
-                     (\<exists>\<sigma> \<sigma>'. s = Normal \<sigma> \<and> t = Normal \<sigma>' \<and> exec_d P \<sigma> = Normal (Some \<sigma>')))"
+  "exec_1_d P = {(s,t). \<exists>\<sigma>. s = Normal \<sigma> \<and> t = TypeError \<and> exec_d P \<sigma> = TypeError} \<union> 
+                {(s,t). \<exists>\<sigma> \<sigma>'. s = Normal \<sigma> \<and> t = Normal \<sigma>' \<and> exec_d P \<sigma> = Normal (Some \<sigma>')}"
 by (auto elim!: exec_1_d.cases intro!: exec_1_d.intros)
 
 
@@ -179,7 +181,7 @@ lemma defensive_imp_aggressive:
 proof -
   have "\<And>x y. P \<turnstile> x -jvmd\<rightarrow> y \<Longrightarrow> \<forall>\<sigma> \<sigma>'. x = Normal \<sigma> \<longrightarrow> y = Normal \<sigma>' \<longrightarrow>  P \<turnstile> \<sigma> -jvm\<rightarrow> \<sigma>'"
     apply (unfold exec_all_d_def1)
-    apply (erule rtrancl_induct')
+    apply (erule rtrancl_induct)
      apply (simp add: exec_all_def)
     apply (fold exec_all_d_def1)
     apply simp
